streams.v
@@ -1,0 +1,48 @@
+(* Copyright (c) 2012-2014, Robbert Krebbers. *)
+(* This file is distributed under the terms of the BSD license. *)
+Require Export tactics.
+
+CoInductive stream (A : Type) : Type := scons : A → stream A → stream A.
+Arguments scons {_} _ _.
+Delimit Scope stream_scope with stream.
+Bind Scope stream_scope with stream.
+Open Scope stream_scope.
+Infix ":.:" := scons (at level 60, right associativity) : stream_scope.
+
+Definition shead {A} (s : stream A) : A := match s with x :.: _ => x end.
+Definition stail {A} (s : stream A) : stream A := match s with _ :.: s => s end.
+
+CoInductive stream_equiv' {A} (s1 s2 : stream A) : Prop :=
+  scons_equiv' :
+    shead s1 = shead s2 → stream_equiv' (stail s1) (stail s2) →
+    stream_equiv' s1 s2.
+Instance stream_equiv {A} : Equiv (stream A) := stream_equiv'.
+
+Reserved Infix "!.!" (at level 20).
+Fixpoint slookup {A} (i : nat) (s : stream A) : A :=
+  match i with O => shead s | S i => stail s !.! i end
+where "s !.! i" := (slookup i s).
+
+Section stream_properties.
+Context {A : Type}.
+Implicit Types x y : A.
+Implicit Types s t : stream A.
+
+Lemma scons_equiv s1 s2 : shead s1 = shead s2 → stail s1 ≡ stail s2 → s1 ≡ s2.
+Proof. by constructor. Qed.
+Global Instance equal_equivalence : Equivalence (@equiv (stream A) _).
+Proof.
+  split.
+  * now cofix; intros [??]; constructor.
+  * now cofix; intros ?? [??]; constructor.
+  * cofix; intros ??? [??] [??]; constructor; etransitivity; eauto.
+Qed.
+Global Instance scons_proper x : Proper ((≡) ==> (≡)) (scons x).
+Proof. by constructor. Qed.
+Global Instance shead_proper : Proper ((≡) ==> (=)) (@shead A).
+Proof. by intros ?? [??]. Qed.
+Global Instance stail_proper : Proper ((≡) ==> (≡)) (@stail A).
+Proof. by intros ?? [??]. Qed.
+Global Instance slookup_proper : Proper ((≡) ==> eq) (@slookup A i).
+Proof. by induction i as [|i IH]; intros s1 s2 Hs; simpl; rewrite Hs. Qed.
+End stream_properties.
